First update law proven

theories/interop/wrapper_wp.v
@@ -4,7 +4,7 @@ From melocoton.mlanguage Require Import mlanguage.
 From melocoton.language Require Import language weakestpre.
 From melocoton.mlanguage Require Import weakestpre.
 From melocoton.interop Require Import wrappersem wrapperstate.
-From iris.base_logic.lib Require Export ghost_map.
+From iris.base_logic.lib Require Export ghost_map ghost_var.
 From iris.algebra.lib Require Import excl_auth gset_bij gmap_view.
 From iris.algebra Require Import ofe.
 From iris.proofmode Require Import proofmode.
@@ -13,23 +13,23 @@ From melocoton.ml_toy_lang Require Import lang melocoton.lang_instantiation  mel
 From melocoton.interop Require Import linking_wp basics.
 Import Wrap.
 
-Print lloc_map.
-Print lstore.
-
-
 Class wrapperGS (hlc : has_lc) Σ := WrapperGS {
   wrapperGS_lstoreGS :> @ghost_mapG Σ lloc block Nat.eq_dec nat_countable;
-  wrapperGS_lloc_mapGS :> @ghost_mapG Σ loc lval loc_eq_decision loc_countable;
-  wrapperGS_locsetGS :> inG Σ (excl_authUR (gsetUR loc));
-  wrapperGS_addrmapGS :> inG Σ (excl_authR (leibnizO addr_map));
+  wrapperGS_freshGS :> @ghost_mapG Σ lloc unit Nat.eq_dec nat_countable;
+  wrapperGS_loc_lvalGS :> @ghost_mapG Σ loc lval loc_eq_decision loc_countable;
+  wrapperGS_lloc_mapGS :> @ghost_mapG Σ loc lloc loc_eq_decision loc_countable;
+  wrapperGS_locsetGS :> ghost_varG Σ (gsetUR loc);
+  wrapperGS_addrmapGS :> ghost_varG Σ (leibnizO addr_map);
+  wrapperGS_at_boundary :> ghost_varG Σ (leibnizO bool);
   wrapperGS_gsetbihGS :> inG Σ (viewR (@gset_bij_view_rel loc loc_eq_decision loc_countable lloc Nat.eq_dec nat_countable));
-  wrapperGS_γζmut : gname;
-  wrapperGS_γζimm : gname;
-  wrapperGS_γζfresh : gname;
+  wrapperGS_γζblock : gname;
+  wrapperGS_γfresh : gname;
   wrapperGS_γroots_set : gname;
   wrapperGS_γroots_map : gname;
   wrapperGS_γθ : gname;
-  wrapperGS_γχ : gname;
+  wrapperGS_γχbij : gname;
+  wrapperGS_γχmap : gname;
+  wrapperGS_γat_boundary : gname;
 }.
 
 Section Embed_logic.
@@ -46,116 +46,339 @@ Implicit Types P : iProp Σ.
 
 Context {WGS : wrapperGS hlc Σ}.
 
-Definition has_mutability (ζ : lstore) (i' : ismut) := forall l i t v, ζ !! l = Some (i,t,v) -> i = i'.
-Definition is_fresh_lstore (χ : lloc_map) (ζ : lstore) : iProp Σ := 
- ∀ (g : lloc) (b:block) (l:loc), ⌜ζ !! g = Some b⌝ → ⌜χ !! l = Some g⌝ → l ↦M/.
-Definition is_mut_lstore (χ : lloc_map) (σ : store) (ζ : lstore) : iProp Σ := 
-   ⌜dom χ = dom σ⌝
- ∗ [∗ map] l ↦ ovl ∈ σ, ∃ (g:lloc) (b:block), ⌜χ !! l = Some g⌝ ∗ ⌜ζ !! g = Some b⌝ ∗ match ovl with
-      None => True (* Blocks owned by C *)
-    | Some vl => True (* TODO: ⌜b ~ vl⌝ *) end (* Blocks in σ, i.e. references *).
-
-Definition gen_lstore_interp (ζ : lstore) (Pmut Pimm Pfresh : lstore → iProp Σ) : iProp Σ := 
-  ∃ ζfresh ζmut ζimm, ⌜ζ = ζfresh ∪ ζmut ∪ ζimm⌝
-         ∗ ghost_map_auth wrapperGS_γζmut 1 ζmut ∗ ⌜has_mutability ζimm Mut⌝ ∗ Pmut ζmut
-         ∗ ghost_map_auth wrapperGS_γζimm 1 ζimm ∗ ⌜has_mutability ζimm Immut⌝ ∗ Pimm ζimm
-         ∗ ghost_map_auth wrapperGS_γζfresh 1 ζfresh ∗ ⌜has_mutability ζimm Mut⌝ ∗ Pfresh ζfresh
-         ∗ ⌜dom ζfresh ## dom ζmut ∧ dom ζfresh ## dom ζimm ∧ dom ζmut ## dom ζimm⌝.
-
-Definition C_lstore_interp (ζ : lstore) (χ : lloc_map) (σvirt : store) : iProp Σ := 
-    gen_lstore_interp ζ
-      (is_mut_lstore χ σvirt)
-      (fun _ => ⌜True⌝)%I
-      (is_fresh_lstore χ).
-
 Definition GC (θ : addr_map) : iProp Σ := 
-   own wrapperGS_γθ (@excl_auth_frag (leibnizO _) θ)
+     ghost_var wrapperGS_γθ (1/2) θ
+   ∗ ghost_var wrapperGS_γat_boundary (1/4) false
    ∗ ∃ (roots : gset addr) (rootsmap : gmap loc lval),
-       own wrapperGS_γroots_set (excl_auth_frag roots)
+       ghost_var wrapperGS_γroots_set (1/2) roots
      ∗ ghost_map_auth wrapperGS_γroots_map 1 rootsmap
      ∗ ⌜dom rootsmap = roots⌝
      ∗ ⌜roots_are_live θ rootsmap⌝
      ∗ ([∗ map] a ↦ v ∈ rootsmap, (∃ w, a ↦C w)).
 
-Definition C_store_interp (ζ : lstore) (χ : lloc_map) (θ : addr_map) (roots : gset addr) : iProp Σ := ∃ σvirt χvirt,
-    C_lstore_interp ζ (χ ∪ χvirt) σvirt
-  ∗ own wrapperGS_γroots_set (excl_auth_auth roots)
-  ∗ (∃ n, state_interp σvirt n)
-  ∗ (own wrapperGS_γχ (gset_bij_auth (DfracOwn 1) (map_to_set pair (χ ∪ χvirt))))
-  ∗ ⌜GC_correct ζ θ⌝.
+Definition block_sim_raw l1 l2 : iProp Σ := (ghost_map_elem (K:=loc) (V:=lloc) wrapperGS_γχmap l1 DfracDiscarded l2).
 
-Definition ML_lstore_interp (ζ : lstore) (χ : lloc_map) : iProp Σ := 
-    gen_lstore_interp ζ
-      (fun ζmut => ⌜ζmut = ∅⌝%I)
-      (fun _ => ⌜True⌝)%I
-      (is_fresh_lstore χ).
+Definition C_state_interp (ζ : lstore) (χ : lloc_map) (θ : addr_map) (roots : gset addr) : iProp Σ :=
+  ∃  (ζfreeze ζσ ζrest : lstore) (χvirt : lloc_map) (fresh : gmap lloc unit) (σMLvirt : store),
+    ghost_var wrapperGS_γroots_set (1/2) roots
+  ∗ ghost_var wrapperGS_γθ (1/2) θ
+  ∗ ghost_map_auth wrapperGS_γζblock 1 ζrest
+  ∗ (∃ n, state_interp σMLvirt n)
+  ∗ own wrapperGS_γχbij (gset_bij_auth (DfracOwn 1) (map_to_set pair χvirt))
+  ∗ ghost_map_auth wrapperGS_γχmap 1 χvirt
+  ∗ ghost_map_auth wrapperGS_γfresh 1 fresh
+  ∗ ([∗ map] ℓ ↦ γ ∈ χvirt, ⌜γ ∈ dom ζrest⌝ -∗ ℓ ↦M/)
+  ∗ ([∗ map] ℓ ↦ γ ∈ χvirt, block_sim_raw ℓ γ)
+  ∗ ([∗ map] l ↦ bb ∈ ζrest, match bb with  (i,t,b) => ⌜i = Immut⌝ -∗ ghost_map_elem (K:=lloc) (V:=block) wrapperGS_γζblock l DfracDiscarded (i,t,b) end)
+  ∗ ghost_var wrapperGS_γat_boundary (1/4) false
+  ∗⌜freeze_lstore ζ ζfreeze
+  ∧ ζfreeze = ζσ ∪ ζrest
+  ∧ dom ζσ ## dom ζrest
+  ∧ is_store_blocks χvirt σMLvirt ζσ
+  ∧ is_store χvirt ζfreeze σMLvirt
+  ∧ lloc_map_mono χ χvirt
+  ∧ gmap_inj χ
+  ∧ (∀ x y, χvirt !! x = Some y → y ∈ dom ζfreeze)
+  ∧ (∀ x y, χvirt !! x = Some y → y ∈ dom fresh → False)
+  ∧ GC_correct ζfreeze θ⌝.
 
 Definition GC_token_remnant (roots : gset addr) : iProp Σ :=
-   own wrapperGS_γθ (@excl_auth_frag (leibnizO _) (∅ : addr_map))
- ∗ own wrapperGS_γroots_set (excl_auth_frag roots)
- ∗ ghost_map_auth wrapperGS_γroots_map 1 (∅ : gmap loc lval)
- ∗ ([∗ set] a ∈ roots, (a O↦ None)). (* Is deallocated in C *)
+   ghost_var wrapperGS_γθ (1/2) (∅:addr_map)
+ ∗ ghost_var wrapperGS_γroots_set (1/2) roots
+ ∗ ghost_map_auth wrapperGS_γroots_map 1 (∅:gmap loc lval)
+ ∗ ([∗ set] a ∈ roots, a O↦ None).
+
+Global Instance ζpers_pers (ζrest : lstore) : Persistent (([∗ map] l ↦ bb ∈ ζrest, match (bb:block) with  (i,t,b) => 
+    ⌜i = Immut⌝ -∗ ghost_map_elem (K:=lloc) (V:=block) wrapperGS_γζblock l DfracDiscarded (i,t,b) end)).
+Proof.
+  apply big_sepM_persistent. intros k ((i&t)&b). apply _.
+Qed.
 
 
-Definition ML_store_interp (ζ : lstore) (χ : lloc_map) (roots : roots_map) (memC : memory) : iProp Σ := 
-    ML_lstore_interp ζ χ
-  ∗ own wrapperGS_γroots_set (excl_auth_auth (dom roots)) ∗ GC_token_remnant (dom roots)
-  ∗ (∃ n, state_interp memC n)
-  ∗ (own wrapperGS_γχ (gset_bij_auth (DfracOwn 1) (map_to_set pair χ))).
+
+Definition ML_state_interp (ζ : lstore) (χ : lloc_map) (roots : roots_map) (memC : memory) : iProp Σ := 
+  ∃  (ζσ ζrest : lstore) (fresh : gmap lloc unit) (σCvirt : memory),
+    ghost_var wrapperGS_γroots_set (1/2) (dom roots)
+  ∗ ghost_var wrapperGS_γθ (1/2) (∅ : addr_map)
+  ∗ ghost_map_auth wrapperGS_γζblock 1 ζrest
+  ∗ (∃ n, state_interp σCvirt n)
+  ∗ own wrapperGS_γχbij (gset_bij_auth (DfracOwn 1) (map_to_set pair χ))
+  ∗ ghost_map_auth wrapperGS_γχmap 1 χ
+  ∗ ghost_map_auth wrapperGS_γfresh (1/2) fresh
+  ∗ ([∗ map] ℓ ↦ γ ∈ χ, ⌜γ ∈ dom ζrest⌝ -∗ ℓ ↦M/)
+  ∗ ([∗ map] ℓ ↦ γ ∈ χ, block_sim_raw ℓ γ)
+  ∗ ([∗ map] l ↦ bb ∈ ζrest, match bb with  (i,t,b) => ⌜i = Immut⌝ -∗ ghost_map_elem (K:=lloc) (V:=block) wrapperGS_γζblock l DfracDiscarded (i,t,b) end)
+  ∗ ghost_var wrapperGS_γat_boundary (1/2) true
+  ∗⌜ζ = ζσ ∪ ζrest
+  ∧ dom ζσ ## dom ζrest
+  ∧ gmap_inj χ
+  ∧ (∀ x y, χ !! x = Some y → y ∈ dom ζ)
+  ∧ (∀ x y, χ !! x = Some y → y ∈ dom fresh → False)⌝.
+
+Definition public_state_interp : store -> iProp Σ := (λ σ, ∃ n, state_interp σ n)%I.
+Definition private_state_interp : wrapstateML -> iProp Σ := (λ ρml, ML_state_interp (ζML ρml) (χML ρml) (rootsML ρml) (privmemML ρml))%I.
 
 Definition wrap_state_interp (σ : Wrap.state) : iProp Σ := match σ with
-  Wrap.CState ρc mem => (∃ n, state_interp mem n) ∗ C_store_interp (ζC ρc) (χC ρc) (θC ρc) (rootsC ρc)
-| Wrap.MLState ρml σ => (∃ n, state_interp σ n) ∗ ML_store_interp (ζML ρml) (χML ρml) (rootsML ρml) (privmemML ρml)
+  Wrap.CState ρc mem => (∃ n, state_interp mem n) ∗ C_state_interp (ζC ρc) (χC ρc) (θC ρc) (rootsC ρc)
+| Wrap.MLState ρml σ => public_state_interp σ ∗ private_state_interp ρml
 end.
 
-(* Old stuff, please ignore
+
+Notation SIC_ip := "((%nCv & HσC) & (%ζfreeze & %ζσ & %ζrest & %χvirt & %fresh & %σMLvirt &
+           HAroots & HAθ & HAζbl & (%nMLv & HAσMLv & HAnMLv) & HAχbij & HAχmap & HAfresh & HAχNone & #HAχpers & #HAζpers & HAbound &
+          %Hfreezeρ & %Hfreezeeq & %Hfreezedj & %Hstore_blocks & %Hstore & %Hχvirt & %Hχinj & %Hfreezeχ & %Hfreshχ & %HGCOK))".
 
 Global Program Instance wrapGS :
   mlanguage.weakestpre.mlangGS hlc _ Σ wrap_lang
 := {
   state_interp := wrap_state_interp;
-  at_boundary := False%I;
+  at_boundary := (ghost_var wrapperGS_γat_boundary (1/2) true)%I;
 }.
 
-Global Program Instance wrap_linkableGS :
-  linkableGS (wrap_lang) (λ σ, ⌜ True ⌝%I)%I
-:= {
-  private_state_interp := (λ _, True)%I;
+Global Program Instance wrap_linkableGS : linkableGS wrap_lang public_state_interp := {
+  private_state_interp := private_state_interp
 }.
-Next Obligation. simpl. intros *. inversion 1. iIntros "?". by iFrame. Qed.
 Next Obligation.
-  simpl. intros ? []. iIntros "? _". iModIntro. iExists _. by iFrame.
+  iIntros (σ pubσ privσ Hlink) "Hσ !>". inversion Hlink; subst. iApply "Hσ".
 Qed.
-Next Obligation. simpl. Print Wrap.split_state. iIntros (σ) "_ Hσ". iPureIntro. exists σ, (). constructor. Qed.
-
-Local Canonical Structure embed_mlang : mlanguage val := lang_to_mlang Λ.
-
-Definition penv_to_mlang (pe : language.weakestpre.prog_environ Λ Σ) :
-  mlanguage.weakestpre.prog_environ (lang_to_mlang Λ) Σ
-:=
-  {| penv_prog := pe.(language.weakestpre.penv_prog);
-     penv_proto := pe.(language.weakestpre.penv_proto) |}.
-
-Lemma wp_embed (e : Λ.(language.expr)) pe E Φ :
-  ⊢ WP e @ pe; E {{ Φ }} -∗ WP e @ (penv_to_mlang pe); E {{ Φ }}.
-Proof using.
-  iStartProof. iLöb as "IH" forall (e). destruct pe as [p T].
-  rewrite {1} @language.weakestpre.wp_unfold /language.weakestpre.wp_pre. simpl.
-  rewrite {1} wp_unfold /mlanguage.weakestpre.wp_pre.
-  iIntros "H" (σ) "(%n & Hσ)". iMod ("H" $! σ n with "Hσ") as "[(%x & %H1 & Hσ & H)|[(%s' & %vv & %K' & %H1 & %H2 & H3)|(%Hred & H3)]]".
-  - iLeft. iModIntro. iExists x. iFrame. iSplitR; first done. iExists n. iFrame.
-  - iRight. iLeft. iMod "H3" as "(%Ξ & Hσ & HT & Hr)". iExists s', vv, K'. iModIntro.
-    iSplitR; first done. iSplitR; first done. iSplitR; first done. iSplitL "Hσ"; first by iExists n.
-    iExists Ξ. iFrame. iNext. iIntros (v) "[Hv _]". iApply "IH". by iApply "Hr".
-  - iRight. iRight. iModIntro. iSplitR.
-    { iPureIntro. destruct Hred as (e' & σ' & H'). eexists (fun '(e2,σ2) => e2 = e' ∧ σ2 = σ'). inversion H'; subst. econstructor. eexists; split; first done.
-      econstructor; first done. intros ? ? ( <- & <- ); done. }
-    iIntros (X Hstep). inversion Hstep as (K & e' & -> & Hx). inversion Hx; subst.
-    unshelve iMod ("H3" $! σ2 _ (Prim_step _ K _ _ _ _ _ _ _ _ _ H3)) as "H3". 1-2:done.
-    do 2 iModIntro. iMod "H3" as "(Hσ & Hwp)". iModIntro. iExists _, _. iSplitR; first (iPureIntro; apply H5; repeat split).
-    iSplitL "Hσ"; first by iExists _. iApply "IH". iApply "Hwp".
+Next Obligation.
+  iIntros (pubσ privσ) "Hpubσ Hprivσ !>".
+  iExists (MLState privσ pubσ). cbn. iSplitL; by iFrame.
+Qed.
+Next Obligation.
+  intros [ρc mem|ρml σ]; cbn; iIntros "Hb Hσ".
+  + iExists _, _. iPureIntro. econstructor.
+  + iExFalso. iAssert (⌜true = false⌝)%I as "%Hdone".
+    * iApply (ghost_var_agree with "Hb [Hσ]").
+      iDestruct "Hσ" as SIC_ip.  iFrame.
+    * iPureIntro. congruence.
 Qed.
 
-*)
+Definition adjoin_mut (m : ismut) (p : tag * list lval) : block := match p with (p1,p2) => (m,p1,p2) end.
+
+Notation "l ↦fresh{ dq } b" := (  ghost_map_elem (K:=lloc) (V:=block) wrapperGS_γζblock l dq (adjoin_mut Mut b)
+                                ∗ ghost_map_elem (K:=lloc) (V:=unit) wrapperGS_γfresh l dq (()))%I
+  (at level 20, format "l  ↦fresh{ dq } b") : bi_scope.
+Notation "l ↦mut{ dq } b" := (  ghost_map_elem (K:=lloc) (V:=block) wrapperGS_γζblock l dq (adjoin_mut Mut b)
+                              ∗ ∃ ll, block_sim_raw ll l)%I
+  (at level 20, format "l  ↦mut{ dq } b") : bi_scope.
+Notation "l ↦imm b" := (  ghost_map_elem (K:=lloc) (V:=block) wrapperGS_γζblock l DfracDiscarded (adjoin_mut Immut b))%I
+  (at level 20, format "l  ↦imm b") : bi_scope.
+
+Fixpoint block_sim (v : MLval) (l : lval) : iProp Σ := match v with
+  (ML_lang.LitV (ML_lang.LitInt x)) => ⌜l = (Lint x)⌝
+| (ML_lang.LitV (ML_lang.LitBool b)) => ⌜l = (Lint (if b then 1 else 0))⌝
+| (ML_lang.LitV ML_lang.LitUnit) => ⌜l = (Lint 0)⌝
+| (ML_lang.LitV ML_lang.LitPoison) => False
+| (ML_lang.LitV (ML_lang.LitLoc ℓ)) => ∃ γ, ⌜l = (Lloc γ)⌝ ∗ block_sim_raw ℓ γ
+| (ML_lang.PairV v1 v2) => ∃ γ lv1 lv2, ⌜l = (Lloc γ)⌝ ∗ γ ↦imm (TagDefault, [lv1;lv2]) ∗ block_sim v1 lv1 ∗ block_sim v2 lv2
+| (ML_lang.InjLV v) => ∃ γ lv, ⌜l = (Lloc γ)⌝ ∗ γ ↦imm (TagDefault, [lv]) ∗ block_sim v lv
+| (ML_lang.InjRV v) => ∃ γ lv, ⌜l = (Lloc γ)⌝ ∗ γ ↦imm (TagInjRV, [lv]) ∗ block_sim v lv 
+| (ML_lang.RecV _ _ _) => False end.
+
+Global Instance block_sim_pers v l : Persistent (block_sim v l).
+Proof.
+  induction v as [[x|b| | |]| | | |] in l|-*; cbn; unshelve eapply (_).
+Qed.
+
+Fixpoint block_sim_arr (v:list MLval) (l : list lval) : iProp Σ := match (v,l) with
+  (nil,nil) => True
+| (v::vr, l::lr) => block_sim v l ∗ block_sim_arr vr lr
+| _ => False end.
+
+Global Instance block_sim_arr_pers vl ll : Persistent (block_sim_arr vl ll).
+Proof.
+  induction vl in ll|-*; destruct ll; cbn; apply _.
+Qed.
+
+Context (σ : Wrap.state).
+Notation SI := (weakestpre.state_interp σ).
+
+
+Lemma GC_in_C {θ}: ⊢ (SI -∗ GC θ -∗ ⌜∃ ρc mem, σ = CState ρc mem⌝)%I.
+Proof.
+  destruct σ. 2: iIntros "_ _"; iPureIntro; do 2 eexists; done.
+  iIntros "((%nCv & HσC) & (%ζσ & %ζrest & %fresh & %σCvirt & HH1 & HH2 & HH3 & HH4 & HH5 & HH6 & HH7 & HH8 & HH9 & HH10 & HH11 & HH12 & HH13))".
+  iIntros "(HG1 & HG2 & HG3)". iExFalso.
+  iAssert (⌜true = false⌝)%I as "%Hdone".
+  1: iApply (ghost_var_agree with "HH11 HG2").
+  congruence.
+Qed.
+
+
+Lemma block_sim_of_ghost_state  (ζfreeze ζσ ζrest : lstore) (χvirt : lloc_map) (σMLvirt : store)
+   v b :
+  ( ([∗ map] ℓ ↦ γ ∈ χvirt, block_sim_raw ℓ γ)
+  ∗ ([∗ map] l ↦ bb ∈ ζrest, match bb with  (i,t,b) => ⌜i = Immut⌝ -∗ ghost_map_elem (K:=lloc) (V:=block) wrapperGS_γζblock l DfracDiscarded (i,t,b) end)
+  ∗⌜
+  ζfreeze = ζσ ∪ ζrest
+∧ is_store_blocks χvirt σMLvirt ζσ
+∧ is_store χvirt ζfreeze σMLvirt
+∧ is_val χvirt ζfreeze v b⌝
+  ) -∗ block_sim v b.
+Proof.
+  iIntros "(H3 & H4 & %H5 & %H7 & %H8 & %HH)".
+  unfold is_store_blocks in H7. unfold is_store in H8.
+  iInduction v as [[x|bo| | |]| | | |] "IH" forall (b HH); cbn; inversion HH; try done.
+  - iExists _. iSplit; first done. iApply (big_sepM_lookup with "H3"); done.
+  - iExists γ, lv1, lv2. iSplit; first done. iSplit.
+    * iApply (big_sepM_lookup _ _ _ (Immut, TagDefault, [lv1; lv2]) with "H4").
+      eapply lookup_union_Some_inv_r. 3: done. 1: subst; apply H1.
+      destruct (ζσ !! γ) eqn:Heq; try done. destruct H7 as [H71 H72].
+      apply elem_of_dom_2 in Heq as Heq2. apply H72 in Heq2.
+      destruct Heq2 as (ll' & C2 & Heq3 & Heq4).
+      specialize (H8 _ _ _ _ Heq4 Heq3 H1). inversion H8.
+    * inversion HH; subst. iSplit. 1: iApply ("IH" with "[] H3 H4"); done. iApply ("IH1" with "[] H3 H4"); done.
+  - iExists γ, lv. iSplit; first done. iSplit.
+    * iApply (big_sepM_lookup _ _ _ (Immut, TagDefault, [lv]) with "H4").
+      eapply lookup_union_Some_inv_r. 3: done. 1: subst; apply H0.
+      destruct (ζσ !! γ) eqn:Heq; try done. destruct H7 as [H71 H72].
+      apply elem_of_dom_2 in Heq as Heq2. apply H72 in Heq2.
+      destruct Heq2 as (ll' & C2 & Heq3 & Heq4).
+      specialize (H8 _ _ _ _ Heq4 Heq3 H0). inversion H8.
+    * iApply ("IH" with "[] H3 H4"); done.
+  - iExists γ, lv. iSplit; first done. iSplit.
+    * iApply (big_sepM_lookup _ _ _ (Immut, TagInjRV, [lv]) with "H4").
+      eapply lookup_union_Some_inv_r. 3: done. 1: subst; apply H0.
+      destruct (ζσ !! γ) eqn:Heq; try done. destruct H7 as [H71 H72].
+      apply elem_of_dom_2 in Heq as Heq2. apply H72 in Heq2.
+      destruct Heq2 as (ll' & C2 & Heq3 & Heq4).
+      specialize (H8 _ _ _ _ Heq4 Heq3 H0). inversion H8.
+    * iApply ("IH" with "[] H3 H4"); done.
+Qed.
+
+Lemma block_sim_arr_of_ghost_state  (ζfreeze ζσ ζrest : lstore) (χvirt : lloc_map) (σMLvirt : store)
+   vs b :
+  ( ([∗ map] ℓ ↦ γ ∈ χvirt, block_sim_raw ℓ γ)
+  ∗ ([∗ map] l ↦ bb ∈ ζrest, match bb with  (i,t,b) => ⌜i = Immut⌝ -∗ ghost_map_elem (K:=lloc) (V:=block) wrapperGS_γζblock l DfracDiscarded (i,t,b) end)
+  ∗⌜
+  ζfreeze = ζσ ∪ ζrest
+∧ is_store_blocks χvirt σMLvirt ζσ
+∧ is_store χvirt ζfreeze σMLvirt
+∧ Forall2 (is_val χvirt ζfreeze) vs b⌝
+  ) -∗ block_sim_arr vs b.
+Proof.
+  iIntros "(H3 & H4 & %H5 & %H7 & %H8 & %H1)".
+  unfold is_store_blocks in H7. unfold is_store in H8.
+  iInduction vs as [|v vs] "IH" forall (b H1).
+  1: apply Forall2_nil_inv_l in H1 as ->; done.
+  destruct b as [|b bs]. 1: by apply Forall2_cons_nil_inv in H1.
+  destruct (Forall2_cons_1 _ _ _ _ _ H1) as [HH H1']. cbn.
+  iSplit.
+  + iApply (block_sim_of_ghost_state with "[H3 H4]"). iFrame. iPureIntro. split; first apply H5. split; first apply H7. split; try done.
+  + iApply ("IH" with "[] H3 H4"); done.
+Qed.
+
+Lemma ml_to_mut θ l vs: ⊢ (SI ∗ GC θ ∗ l ↦∗ vs ==∗ SI ∗ GC θ ∗ ∃ b γ, γ ↦mut{DfracOwn 1} (TagDefault,b) ∗ block_sim_raw l γ ∗ block_sim_arr vs b)%I.
+Proof.
+  iIntros "(Hσ & HGC & Hl)".
+  iDestruct (GC_in_C with "Hσ HGC") as "%H"; destruct H as (ρc & mem & ->).
+  iDestruct "Hσ" as SIC_ip.
+  unfold state_interp. cbn.
+  iDestruct (gen_heap_valid with "HAσMLv Hl") as %Hlσ.
+  destruct (χvirt !! l) as [ll|] eqn:Hlχ.
+  2: { exfalso. 
+       apply not_elem_of_dom_2 in Hlχ.
+       apply elem_of_dom_2 in Hlσ.
+       destruct Hstore_blocks as [Hdom Hstore_blocks]. unfold lloc_map in Hdom. rewrite <- Hdom in Hlχ.
+       by apply Hlχ. }
+  iMod (gen_heap_update _ _ _ None with "HAσMLv Hl") as "[HAσMLv Hl]".
+  assert (ll ∈ dom ζσ) as Hllζ.
+  1: { destruct Hstore_blocks as [Hdom Hstore_blocks]. apply Hstore_blocks. exists l, vs. split; try done. }
+  apply elem_of_dom in Hllζ. destruct Hllζ as [bb Hζσll].
+  iMod (ghost_map_insert _ bb with "HAζbl") as "(HAζbl & Hzz)".
+  1: { edestruct @elem_of_disjoint as [eodj _]. specialize (eodj Hfreezedj).
+       apply not_elem_of_dom. refine (eodj ll _). apply elem_of_dom. done. }
+  iModIntro. iFrame "HGC".
+  unfold is_store in Hstore.
+  assert (ζfreeze !! ll = Some bb) as Hfreezell.
+  1: { rewrite Hfreezeeq. rewrite lookup_union. rewrite Hζσll. unfold union_with. cbn.
+       destruct (ζrest !! ll) eqn:Heq; rewrite Heq; done. }
+  specialize (Hstore l vs ll bb Hlσ Hlχ Hfreezell) as Hstorel.
+  inversion Hstorel; subst vs0 bb.
+  iAssert (block_sim_arr vs lvs) as "#Hblock".
+  1: { iApply (block_sim_arr_of_ghost_state). iSplitR; first iApply "HAχpers". iSplitR; first iApply "HAζpers".
+       iPureIntro. split; first apply Hfreezeeq. split; first eauto. split; eauto. }
+  iAssert (block_sim_raw l ll) as "#Hraw".
+  1: iApply (big_sepM_lookup with "HAχpers"); done.
+  iAssert (⌜gset_bijective (map_to_set pair χvirt)⌝)%I as "%Hbij".
+  1: { iPoseProof (own_valid with "HAχbij") as "%Hvalid". apply gset_bij_auth_valid in Hvalid. done. }
+  iSplitR "Hzz". 1: iSplitL "HσC".
+  + iExists _. iApply "HσC".
+  + unfold C_state_interp. iExists (ζfreeze), (delete ll ζσ), (<[ll:=(Mut, TagDefault, lvs)]> ζrest).
+    iExists χvirt, fresh, (<[l:=None]> σMLvirt). iFrame.
+    iSplitL "HAnMLv". 1: iExists _; iFrame.
+    iSplitL. 
+    1: {assert (χvirt = <[ l := ll ]> (delete l χvirt)) as Hχeq.
+        + apply map_eq_iff. intros i. destruct (decide (i = l)); subst. 1: by rewrite lookup_insert.
+          rewrite lookup_insert_ne. 1: rewrite lookup_delete_ne. all: done.
+        + iPoseProof (big_sepM_delete _ _ _ _ Hlχ) as "(Hdel & _)". iPoseProof ("Hdel" with "HAχNone") as "(_ & Hdel')".
+          rewrite {5} Hχeq. iApply (big_sepM_insert_2 with "[Hl]"). 1: iIntros "_"; done.
+          iApply (big_sepM_impl with "Hdel'"). iIntros "%k %v %Hdeleq !>  Hin %Hdom".
+          iApply "Hin". iPureIntro. apply elem_of_dom. apply elem_of_dom in Hdom. destruct Hdom as [x Hx]. destruct (decide (v = ll)).
+          2: exists x; rewrite lookup_insert_ne in Hx; done.
+          subst v. apply lookup_delete_Some in Hdeleq. destruct Hdeleq as [Hdelne Hkχ].
+          enough (l = k) by congruence. eapply gset_bijective_eq_iff. 1: apply Hbij.
+          1-2: by apply elem_of_map_to_set_pair. done. 
+        }
+    iSplitL; first iApply "HAχpers". iSplitL.
+    1: { iApply big_sepM_insert.
+         + apply not_elem_of_dom. apply elem_of_dom_2 in Hζσll.
+           edestruct @elem_of_disjoint as [eodj _]. specialize (eodj Hfreezedj).
+           exact (eodj _ Hζσll).
+         + iSplit. 2: iApply "HAζpers". iIntros "%Hne"; congruence. }
+    iPureIntro. split; last split; last split; last split; last split; last split; last split; last split; last split.
+    all: try done; eauto.
+    - symmetry. subst. by apply union_delete_insert.
+    - apply map_disjoint_dom_1. apply map_disjoint_insert_r_2. 1: apply lookup_delete.
+      apply map_disjoint_delete_l. apply map_disjoint_dom_2. done.
+    - destruct Hstore_blocks as [HL HR]. split.
+      1: rewrite dom_insert_lookup_L; try done. intros ll'.
+      destruct (decide (ll' = ll)); try subst ll'; split.
+      * intros [x Hx]%elem_of_dom. rewrite lookup_delete in Hx. done.
+      * intros (ℓ & Vs & HH1 & HH2).
+        enough (l = ℓ) as <-. 2: eapply gset_bijective_eq_iff. 2: apply Hbij.
+        2-3: by apply elem_of_map_to_set_pair. 2: done.
+        rewrite lookup_insert in HH2. done.
+      * intros [x Hx]%elem_of_dom. rewrite lookup_delete_ne in Hx. 2:done. 
+        destruct (HR ll') as [(ℓ & Vs & HH1 & HH2) _].  1: by apply elem_of_dom.
+        exists ℓ, Vs. split; first done.
+        rewrite lookup_insert_ne; try done. intros Hn.
+        eapply (gset_bijective_eq_iff _ _ _ _ _ Hbij) in Hn. 1: apply n; symmetry; apply Hn. 
+        all: by apply elem_of_map_to_set_pair.
+      * intros (ℓ & Vs & HH1 & HH2). apply elem_of_dom. rewrite lookup_delete_ne; last done.
+        apply elem_of_dom.
+        destruct (HR ll') as [_ Hdom]. apply Hdom.
+        exists ℓ, Vs; split; try done.
+        rewrite lookup_insert_ne in HH2; try done. intros Hn.
+        eapply (gset_bijective_eq_iff _ _ _ _ _ Hbij) in Hn. 1: apply n; symmetry; apply Hn. 
+        all: by apply elem_of_map_to_set_pair.
+    - intros ℓ Vs γ blk HH1 HH2 HH3. eapply Hstore; try done. destruct (decide (ℓ = l)).
+      1: subst ℓ; rewrite lookup_insert in HH1; done.
+      rewrite lookup_insert_ne in HH1; try done.
+  + iExists lvs, ll. iFrame. iFrame "Hblock". unfold block_sim_raw.
+    iSplit; first iExists l. all: iApply  "Hraw".
+Qed.
 
 End Embed_logic.
+
+
+
+
+
+
+
+
+
+
+
+
+
+
+
+
+
+
+
+
+
